propagate step 1

src/Std/Tactic/BVDecide/Bitblast/BVExpr/Circuit/Impl/Pred.lean
@@ -21,15 +21,12 @@ open Std.Sat
 namespace BVPred
 
 def bitblast (aig : AIG BVBit) (pred : BVPred) : AIG.Entrypoint BVBit :=
+  let cache := BVExpr.Cache.empty
   match pred with
   | .bin lhs op rhs =>
-    let res := lhs.bitblast aig
-    let aig := res.aig
-    let lhsRefs := res.vec
-    let res := rhs.bitblast aig
-    let aig := res.aig
-    let rhsRefs := res.vec
-    let lhsRefs := lhsRefs.cast <| AIG.LawfulVecOperator.le_size (f := BVExpr.bitblast) ..
+    let ⟨⟨⟨aig, lhsRefs⟩, _⟩, cache⟩ := BVExpr.bitblast aig ⟨lhs, cache⟩
+    let ⟨⟨⟨aig, rhsRefs⟩, hrhs⟩, _⟩ := BVExpr.bitblast aig ⟨rhs, cache⟩
+    let lhsRefs := lhsRefs.cast hrhs
     match op with
     | .eq => mkEq aig ⟨lhsRefs, rhsRefs⟩
     | .ult => mkUlt aig ⟨lhsRefs, rhsRefs⟩
@@ -39,59 +36,61 @@ def bitblast (aig : AIG BVBit) (pred : BVPred) : AIG.Entrypoint BVBit :=
     However the vast majority of operations are interested in all bits so the API is currently
     not designed to support this use case.
     -/
-    let res := expr.bitblast aig
-    let aig := res.aig
-    let refs := res.vec
+    let ⟨⟨⟨aig, refs⟩, _⟩, _⟩ := BVExpr.bitblast aig ⟨expr, cache⟩
     blastGetLsbD aig ⟨refs, idx⟩
 
 instance : AIG.LawfulOperator BVBit (fun _ => BVPred) bitblast where
   le_size := by
     intro aig pred
-    unfold bitblast
+    unfold BVPred.bitblast
     cases pred with
     | bin lhs op rhs =>
       cases op with
       | eq =>
+        dsimp only
         apply AIG.LawfulOperator.le_size_of_le_aig_size (f := mkEq)
-        apply AIG.LawfulVecOperator.le_size_of_le_aig_size (f := BVExpr.bitblast)
-        apply AIG.LawfulVecOperator.le_size (f := BVExpr.bitblast)
+        refine Nat.le_trans ?_ (BVExpr.bitblast_le_size ..)
+        apply BVExpr.bitblast_le_size
       | ult =>
+        dsimp only
         apply AIG.LawfulOperator.le_size_of_le_aig_size (f := mkUlt)
-        apply AIG.LawfulVecOperator.le_size_of_le_aig_size (f := BVExpr.bitblast)
-        apply AIG.LawfulVecOperator.le_size (f := BVExpr.bitblast)
+        refine Nat.le_trans ?_ (BVExpr.bitblast_le_size ..)
+        apply BVExpr.bitblast_le_size
     | getLsbD expr idx =>
+      dsimp only
       apply AIG.LawfulOperator.le_size_of_le_aig_size (f := blastGetLsbD)
-      apply AIG.LawfulVecOperator.le_size (f := BVExpr.bitblast)
+      apply BVExpr.bitblast_le_size
   decl_eq := by
     intro aig pred idx h1 h2
+    unfold BVPred.bitblast
     cases pred with
     | bin lhs op rhs =>
       cases op with
       | eq =>
-        simp only [bitblast]
+        dsimp only
         rw [AIG.LawfulOperator.decl_eq (f := mkEq)]
-        rw [AIG.LawfulVecOperator.decl_eq (f := BVExpr.bitblast)]
-        rw [AIG.LawfulVecOperator.decl_eq (f := BVExpr.bitblast)]
-        · apply AIG.LawfulVecOperator.lt_size_of_lt_aig_size (f := BVExpr.bitblast)
+        rw [BVExpr.bitblast_decl_eq]
+        rw [BVExpr.bitblast_decl_eq]
+        · apply BVExpr.bitblast_lt_size_of_lt_aig_size
           assumption
-        · apply AIG.LawfulVecOperator.lt_size_of_lt_aig_size (f := BVExpr.bitblast)
-          apply AIG.LawfulVecOperator.le_size_of_le_aig_size (f := BVExpr.bitblast)
+        · apply BVExpr.bitblast_lt_size_of_lt_aig_size
+          apply BVExpr.bitblast_lt_size_of_lt_aig_size
           assumption
       | ult =>
         simp only [bitblast]
         rw [AIG.LawfulOperator.decl_eq (f := mkUlt)]
-        rw [AIG.LawfulVecOperator.decl_eq (f := BVExpr.bitblast)]
-        rw [AIG.LawfulVecOperator.decl_eq (f := BVExpr.bitblast)]
-        · apply AIG.LawfulVecOperator.lt_size_of_lt_aig_size (f := BVExpr.bitblast)
+        rw [BVExpr.bitblast_decl_eq]
+        rw [BVExpr.bitblast_decl_eq]
+        · apply BVExpr.bitblast_lt_size_of_lt_aig_size
           assumption
-        · apply AIG.LawfulVecOperator.lt_size_of_lt_aig_size (f := BVExpr.bitblast)
-          apply AIG.LawfulVecOperator.le_size_of_le_aig_size (f := BVExpr.bitblast)
+        · apply BVExpr.bitblast_lt_size_of_lt_aig_size
+          apply BVExpr.bitblast_lt_size_of_lt_aig_size
           assumption
     | getLsbD expr idx =>
       simp only [bitblast]
       rw [AIG.LawfulOperator.decl_eq (f := blastGetLsbD)]
-      rw [AIG.LawfulVecOperator.decl_eq (f := BVExpr.bitblast)]
-      apply AIG.LawfulVecOperator.lt_size_of_lt_aig_size (f := BVExpr.bitblast)
+      rw [BVExpr.bitblast_decl_eq]
+      apply BVExpr.bitblast_lt_size_of_lt_aig_size
       assumption
 
 end BVPred
